backup (refined a21, a22, a23, started 3.21

process/beta.v
@@ -59,16 +59,13 @@ Definition subst_expr_proc (p : process) (lb : label) (e : expr) : (option proce
 
 Inductive betaP: relation session :=
   | r_comm  : forall p q xs l e Q M,
-              betaP ((p <-- Some (p_recv q xs)) ||| (q <-- Some (p_send p l e Q)) ||| M)
-                    ((p <-- subst_expr_proc (p_recv q xs) l e) ||| (q <-- Some Q) ||| M)
+              betaP ((p <-- (p_recv q xs)) ||| (q <-- (p_send p l e Q)) ||| M)
+                    ((p <-- subst_expr_proc (p_recv q xs) l e) ||| (q <-- Q) ||| M)
   | rt_ite  : forall p P Q M,
-              betaP ((p <-- Some (p_ite (e_val (vbool true)) P Q)) ||| M) ((p <-- Some P) ||| M)
+              betaP ((p <-- (p_ite (e_val (vbool true)) P Q)) ||| M) ((p <-- P) ||| M)
   | rf_ite  : forall p P Q M,
-              betaP ((p <-- Some (p_ite (e_val (vbool false)) P Q)) ||| M) ((p <-- Some Q) ||| M)
+              betaP ((p <-- (p_ite (e_val (vbool false)) P Q)) ||| M) ((p <-- Q) ||| M)
   | r_struct: forall M1 M1' M2 M2', scong M1 M1' -> scong M2' M2 -> betaP M1' M2' -> betaP M1 M2.
-
-Declare Instance Equivalence_beta : Equivalence betaP.
-
 
 Definition beta_multistep := multi betaP.
 
@@ -91,7 +88,7 @@ Definition MS: session := ("Alice" <-- Some PAlice) ||| ("Bob" <-- Some PBob) ||
 Definition MS': session := ("Alice" <-- Some p_inact) ||| ("Bob" <-- Some p_inact) ||| ("Carol" <-- Some p_inact).
 
 Eval compute in (eval_expr (e_plus (e_val (vint 100)) (e_val (vint 5)))).
-
+(* 
 Example redMS: beta_multistep MS MS'.
 Proof. unfold beta_multistep, MS, MS', PAlice, PBob.
 
@@ -124,5 +121,5 @@ Proof. unfold beta_multistep, MS, MS', PAlice, PBob.
        apply r_comm.
        apply multi_refl.
 Qed.
-
+ *)
 
