process/sessions.v
@@ -1,34 +1,271 @@
-From SST Require Export src.unscoped src.expressions process.processes type.global tree.global.
-Require Import List String Relations.
-Require Import List String Relations ZArith.
+From SST Require Export src.unscoped src.expressions process.processes process.substitution process.inversion process.typecheck type.global type.local tree.global tree.local.
+Require Import List String Datatypes ZArith Relations PeanoNat.
+Open Scope list_scope.
 Require Import Setoid Morphisms Coq.Program.Basics.
 Require Import Coq.Init.Datatypes.
 
 Inductive session: Type :=
-  | s_ind : part   -> option process -> session
-  | s_par: session -> session -> session.
+  | s_ind : part   -> process -> session
+  | s_par : session -> session -> session.
   
-
-(* Inductive pcong: relation process :=
-  | pc_rec  : forall p, pcong (p_rec p) (subst_process ((p_rec p) .: p_var) p). *)
-
 Notation "p '<--' P"   :=  (s_ind p P) (at level 50, no associativity).
 Notation "s1 '|||' s2" :=  (s_par s1 s2) (at level 50, no associativity).
+  
+(* Inductive sForall (P: session -> Prop) : session -> Prop :=
+  | fsind: forall p proc, sForall P (p <-- proc)
+  | fspar: forall (S R: session), P S -> P R -> sForall P (S ||| R).
+ *)
+ 
+Print Forall.
 
+Inductive ForallT (P : part -> process -> Prop) : session -> Prop := 
+  | ForallT_mono : forall pt op, P pt op -> ForallT P (pt <-- op)
+  | ForallT_par : forall (M1 M2 : session), ForallT P M1 -> ForallT P M2 -> ForallT P (M1 ||| M2). 
+  
+
+Fixpoint InT (pt : part) (M : session) : Prop :=
+  match M with 
+    | p <-- _ => p = pt 
+    | M1 |||  M2 => (InT pt M1) \/ (InT pt M2)
+  end.
+
+Inductive typ_sess : session -> gtt -> Prop := 
+  | t_sess : forall M G, (forall pt, isgPartsC pt G -> InT pt M) ->
+                         ForallT (fun u P => exists T, projectionC G u T /\ typ_proc nil nil P T) M ->
+                         typ_sess M G.
+
+Lemma _a23_2 : forall M G, typ_sess M G -> (forall pt, isgPartsC pt G -> InT pt M) /\ 
+               ForallT (fun u P => exists T, projectionC G u T /\ typ_proc nil nil P T) M.
+Proof.
+  intros. inversion H; try easy.
+Qed.
+
+(* not done *)
+Inductive stepE : relation expr := 
+  | ec_var   : forall n, stepE (e_var n) (e_var n)
+  | ec_val   : forall v, stepE (e_val v) (e_val v)
+  | ec_succ  : forall n, stepE (e_succ (e_val (vint n))) (e_val (vint (n+1))).
+   
 Inductive scongP : relation process := 
-  | pc_rec : forall P Q, substitutionP 0 0 0 (p_rec P) P Q -> scongP (p_rec P) Q.
+  | pc_inact : scongP p_inact p_inact
+  | pc_var   : forall n, scongP (p_var n) (p_var n)
+  | pc_mu    : forall X Y, scongP X Y -> scongP (p_rec X) (p_rec Y)
+  | pc_ite   : forall e e' X X' Y Y', stepE e e' -> scongP X X' -> scongP Y Y' -> scongP (p_ite e X Y) (p_ite e' X' Y')
+  | pc_recv  : forall pt xs ys, Forall2 (fun u v => (u = None /\ v = None) \/ (exists P Q, u = Some P /\ v = Some Q /\ scongP P Q)) xs ys -> scongP (p_recv pt xs) (p_recv pt ys)
+  | pc_send  : forall pt lb e e' X X', stepE e e' -> scongP X X' -> scongP (p_send pt lb e X) (p_send pt lb e' X')
+  | pc_sub   : forall P Q, substitutionP 0 0 0 (p_rec P) P Q -> scongP (p_rec P) Q
+  | pc_trans : forall P Q R, scongP P Q -> scongP Q R -> scongP P R.
 
+Section scongP_ind_ref.
+  Variable P : process -> process -> Prop.
+  Hypothesis P_inact : P p_inact p_inact.
+  Hypothesis P_var   : forall n, P (p_var n) (p_var n).
+  Hypothesis P_mu    : forall X Y, P X Y -> P (p_rec X) (p_rec Y).
+  Hypothesis P_ite   : forall e e' X X' Y Y', stepE e e' -> P X X' -> P Y Y' -> P (p_ite e X Y) (p_ite e' X' Y').
+  Hypothesis P_recv  : forall pt xs ys, Forall2 (fun u v => (u = None /\ v = None) \/ (exists X Y, u = Some X /\ v = Some Y /\ P X Y)) xs ys -> P (p_recv pt xs) (p_recv pt ys).
+  Hypothesis P_send  : forall pt lb e e' X X', stepE e e' -> P X X' -> P (p_send pt lb e X) (p_send pt lb e' X').
+  Hypothesis P_sub   : forall X Y, substitutionP 0 0 0 (p_rec X) X Y -> P (p_rec X) Y.
+  Hypothesis P_trans : forall X Y Z, P X Y -> P Y Z -> P X Z.
+  
+  Fixpoint scongP_ind_ref (X Y : process) (a : scongP X Y) {struct a} : P X Y.
+  Proof.
+    refine (match a with
+      | pc_inact => P_inact
+      | pc_var n => P_var n 
+      | pc_mu X Y Hp => P_mu X Y (scongP_ind_ref X Y Hp)
+      | pc_ite e e' X X' Y Y' He Hx Hy => P_ite e e' X X' Y Y' He (scongP_ind_ref X X' Hx) (scongP_ind_ref Y Y' Hy)
+      | pc_recv pt xs ys Ha => P_recv pt xs ys _
+      | pc_send pt lb e e' X X' He Hx => P_send pt lb e e' X X' He (scongP_ind_ref X X' Hx)
+      | pc_sub X Y Hs => P_sub X Y Hs
+      | pc_trans X Y Z Hxy Hyz => P_trans X Y Z (scongP_ind_ref X Y Hxy) (scongP_ind_ref Y Z Hyz)
+    end); try easy.
+    revert Ha. apply Forall2_mono. intros.
+    destruct H. left. easy.
+    destruct H. destruct H. destruct H. destruct H0. subst. right.
+    exists x0. exists x1. split; try easy. split; try easy.
+    apply scongP_ind_ref; try easy.
+  Qed.
+End scongP_ind_ref.
 
 Inductive scong: relation session :=
-  | sc_multi: forall p P Q M, scongP P Q -> scong (p <-- Some P ||| M) (p <-- Some Q ||| M) 
-  | sc_par1 : forall p M, scong (p <-- Some p_inact ||| M) M
+  | sc_multi: forall p P Q M, scongP P Q -> scong (p <-- P ||| M) (p <-- Q ||| M) 
+  | sc_par1 : forall p M, scong (p <-- p_inact ||| M) M
   | sc_par2 : forall M M', scong (M ||| M') (M' ||| M)
-  | sc_par3 : forall M M' M'', scong ((M ||| M') ||| M'') (M ||| (M' ||| M''))
-  | sc_par4 : forall M M' M'', scong ((M ||| M') ||| M'') (M ||| (M'' ||| M')).
+  | sc_par3 : forall M M' M'', scong ((M ||| M') ||| M'') (M ||| (M' ||| M'')).
 
-Declare Instance Equivalence_pcong : Equivalence scongP. 
+Lemma _a22_2_helper : forall pt G, isgPartsC pt G -> projectionC G pt ltt_end -> False.
+Admitted.
+
+Lemma expr_typ_cong : forall Gs e e' S, typ_expr Gs e S -> stepE e e' -> typ_expr Gs e' S.
+Proof.
+Admitted.
+
+Lemma _a22_2_helperP_1 : forall xs x l' Gs Gt,
+      Forall2
+       (fun u v : option process =>
+        u = None /\ v = None \/
+        (exists X Y : process,
+           u = Some X /\
+           v = Some Y /\
+           (forall (Gs : ctxS) (Gt : ctxT) (T : ltt), typ_proc Gs Gt X T -> typ_proc Gs Gt Y T))) xs l' ->
+      Forall2
+        (fun (u : option process) (v : option (sort * ltt)) =>
+         u = None /\ v = None \/
+         (exists (p : process) (s : sort) (t : ltt),
+            u = Some p /\ v = Some (s, t) /\ typ_proc (Some s :: Gs) Gt p t)) xs x ->
+      Forall2
+      (fun (u : option process) (v : option (sort * ltt)) =>
+       u = None /\ v = None \/
+       (exists (p : process) (s : sort) (t : ltt),
+          u = Some p /\ v = Some (s, t) /\ typ_proc (Some s :: Gs) Gt p t)) l' x.
+Proof.
+  intro xs. induction xs; intros; try easy.
+  inversion H. subst. inversion H0. subst. easy.
+  inversion H. subst. inversion H0. subst. clear H H0.
+  constructor. destruct H3. left. destruct H4; try easy.
+  destruct H. destruct H0. destruct H0. destruct H0. destruct H0. subst. easy.
+  right. destruct H. destruct H. destruct H. destruct H0. subst.
+  exists x0. destruct H4. easy. destruct H. destruct H. destruct H. destruct H. destruct H0. subst.
+  exists x2. exists x3. split; try easy. split; try easy.
+  apply H1. inversion H. subst. easy.
+  apply IHxs; try easy.
+Qed.
+
+Lemma _a22_2_helperP_2 : forall xs l',
+      SList xs ->
+      Forall2
+       (fun u v : option process =>
+        u = None /\ v = None \/
+        (exists X Y : process,
+           u = Some X /\
+           v = Some Y /\
+           (forall (Gs : ctxS) (Gt : ctxT) (T : ltt), typ_proc Gs Gt X T -> typ_proc Gs Gt Y T))) xs l' ->
+      SList l'.
+Proof.
+  intro xs. induction xs; intros; try easy.
+  inversion H0. subst. 
+  specialize(SList_f a xs H); intros. destruct H1.
+  - apply SList_b. apply IHxs; try easy.
+  - destruct H1. destruct H2. subst. inversion H5. subst. destruct H3; try easy.
+    destruct H1. destruct H1. destruct H1. destruct H2. subst. easy.
+Qed.
+  
+Lemma _a22_2_helperP_h : forall Gs Gt pt xs ys T,
+    typ_proc Gs Gt (p_recv pt xs) T ->
+    Forall2
+      (fun u v : option process =>
+       u = None /\ v = None \/
+       (exists X Y : process,
+          u = Some X /\
+          v = Some Y /\
+          (forall (Gs : ctxS) (Gt : ctxT) (T : ltt), typ_proc Gs Gt X T -> typ_proc Gs Gt Y T))) xs ys ->
+    typ_proc Gs Gt (p_recv pt ys) T.
+Proof.
+  intros Gs Gt pt xs. revert Gs Gt pt.
+  induction xs; intros; try easy.
+  - inversion H0. subst. easy.
+  - inversion H0. subst. clear H0.
+    specialize(_a23_a pt (a :: xs) (p_recv pt (a :: xs)) Gs Gt T H (eq_refl (p_recv pt (a :: xs)))); intros.
+    destruct H0. destruct H0. destruct H1. destruct H2.
+    apply tc_sub with (t := ltt_recv pt x); try easy.
+    destruct x; try easy.
+    apply tc_recv; try easy.
+    simpl. apply eq_S.
+    inversion H0.
+    specialize(Forall2_length H5); intros. easy.
+    specialize(SList_f a xs H4); intros. clear H4. destruct H6.
+    - apply SList_b.
+      apply _a22_2_helperP_2 with (xs := xs); try easy.
+    - destruct H4. destruct H6. subst. destruct H3; try easy.
+      destruct H3. destruct H3. destruct H3. destruct H4. inversion H3. subst.
+      inversion H5. subst. easy.
+    - constructor. 
+      destruct H3. left. destruct H3. inversion H2. subst.
+      destruct H10. easy. destruct H3. destruct H3. destruct H3. easy.
+      right.
+      destruct H3. destruct H3. destruct H3. destruct H6. 
+      exists x1.
+      inversion H2; subst. destruct H11; try easy.
+      destruct H3. destruct H3. destruct H3. destruct H3. destruct H6. subst.
+      exists x3. exists x4.
+      split; try easy. split; try easy. 
+      apply H7. inversion H3. subst. easy.
+    - inversion H2. subst. clear H2.
+      apply _a22_2_helperP_1 with (xs := xs); try easy.
+      apply typable_implies_wfC with (P := (p_recv pt (a :: xs))) (Gs := Gs) (Gt := Gt); try easy.
+Qed.
+
+Lemma _a22_2_helperP : forall Gs Gt P Q T, typ_proc Gs Gt P T -> scongP P Q -> typ_proc Gs Gt Q T.
+Proof.
+  intros. revert H. revert Gs Gt T.
+  induction H0 using scongP_ind_ref; intros; try easy.
+  - specialize(_a23_d (p_rec X) X T Gs Gt H (eq_refl (p_rec X))); intros.
+    destruct H0. destruct H0. 
+    specialize(IHscongP Gs (Some x :: Gt) x H0).
+    apply tc_sub with (t := x); try easy.
+    apply tc_mu; try easy.
+    apply typable_implies_wfC with (P := p_rec X) (Gs := Gs) (Gt := Gt); try easy.
+  - specialize(_a23_c (p_ite e X Y) e X Y T Gs Gt H0 (eq_refl (p_ite e X Y))); intros.
+    destruct H1. destruct H1. destruct H1. destruct H2. destruct H3. destruct H4.
+    apply tc_ite.
+    apply expr_typ_cong with (e := e); try easy.
+    apply IHscongP; try easy. apply tc_sub with (t := x); try easy.
+    apply typable_implies_wfC with (P := p_ite e X Y) (Gs := Gs) (Gt := Gt); try easy.
+    apply IHscongP0; try easy. apply tc_sub with (t := x0); try easy.
+    apply typable_implies_wfC with (P := p_ite e X Y) (Gs := Gs) (Gt := Gt); try easy.
+  - apply _a22_2_helperP_h with (xs := xs); try easy.
+  - specialize(_a23_bf pt lb e X (p_send pt lb e X) Gs Gt T H0 (eq_refl (p_send pt lb e X))); intros.
+    destruct H1. destruct H1. destruct H1. destruct H2.
+    apply tc_sub with (t := (ltt_send pt (extendLTT lb nil (Some (x, x0))))); try easy.
+    apply tc_send; try easy.
+    apply expr_typ_cong with (e := e); try easy.
+    apply IHscongP; try easy.
+    apply typable_implies_wfC with (P := p_send pt lb e X) (Gs := Gs) (Gt := Gt). easy.
+  - specialize(_a23_d (p_rec X) X T Gs Gt H0 (eq_refl (p_rec X))); intros.
+    destruct H1. destruct H1.  
+    specialize(_a21f X (p_rec X)); intros.
+    apply tc_sub with (t := x); intros; try easy.
+    apply H3 with (T := x); try easy.
+    apply tc_mu; intros; try easy.
+    apply typable_implies_wfC with (P := p_rec X) (Gs := Gs) (Gt := Gt); try easy.
+  - apply IHscongP0; try easy. apply IHscongP; try easy.
+Qed.
+
+
+Lemma _a22_2 : forall M M' G, typ_sess M G -> scong M M' -> typ_sess M' G.
+Proof.
+  intros. revert H. revert G. induction H0; intros; try easy.
+  - inversion H0. subst. inversion H2. subst. clear H2.
+    inversion H5. subst. clear H5. destruct H3. destruct H2.
+    constructor; try easy. constructor; try easy. constructor; try easy. 
+    exists x. split; try easy.
+    apply _a22_2_helperP with (P := P); try easy.
+  - inversion H. subst. inversion H1. subst. clear H1. 
+    constructor; try easy.
+    intros. specialize(H0 pt H1).
+    simpl in H0. destruct H0; try easy. subst. 
+    inversion H4. subst. destruct H2. destruct H0.
+    specialize(_a23_f p_inact x nil nil H2 (eq_refl p_inact)); intros. subst. clear H4 H5 H2.
+    specialize(_a22_2_helper pt G H1 H0); intros. easy.
+  - inversion H; subst. inversion H1; subst. constructor.
+    intros. specialize (H0 pt H2); intros. simpl. 
+    destruct H0; try easy. right. easy. left. easy.
+    constructor; try easy.
+  - inversion H; subst. inversion H1; subst. inversion H4; subst. clear H1 H4.
+    constructor. 
+    - intros. specialize(H0 pt H1). simpl in *. 
+      destruct H0. destruct H0. left. easy. 
+      right. left. easy.
+      right. right. easy.
+    constructor; try easy. constructor; try easy.
+Qed.
+
+
+
+(* Declare Instance Equivalence_pcong : Equivalence scongP. 
 Declare Instance Equivalence_scong : Equivalence scong.
 
 Inductive sForall (P: session -> Prop): session -> Prop :=
   | fsind: forall p proc, sForall P (p <-- proc)
   | fspar: forall (S R: session), P S -> P R -> sForall P (S ||| R).
+ *)
