process/subject_reduction.v
@@ -1,0 +1,66 @@
+From SST Require Export src.unscoped src.expressions process.processes process.typecheck type.global type.local tree.global tree.local process.beta process.sessions process.inversion.
+Require Import List String Datatypes ZArith Relations PeanoNat.
+Open Scope list_scope.
+Require Import Setoid Morphisms Coq.Program.Basics.
+Require Import Coq.Init.Datatypes.
+
+Inductive multiC : relation gtt := 
+  | multiC_refl : forall G, multiC G G
+  | multiC_step : forall G1 G2 G3 p q n, gttstepC G1 G2 p q n -> multiC G2 G3 -> multiC G1 G3.
+
+
+
+Theorem _3_21 : forall M M' G, typ_sess M G -> betaP M M' -> exists G', typ_sess M' G' /\ multiC G G'.
+Proof.
+  intros. revert H. revert G.
+  induction H0; intros; try easy.
+  (* R-COMM *)
+  inversion H. subst. inversion H1. subst. clear H1. inversion H4. subst. clear H4.
+  inversion H3. subst. clear H3. inversion H6. subst. clear H6.
+  - destruct H2. destruct H1. destruct H1. destruct H2. inversion H2. subst. clear H2.
+    destruct H3. destruct H2. destruct H2. destruct H3. inversion H3. subst. clear H3.
+  - specialize(_a23_a q xs (p_recv q xs) nil nil x H4 (eq_refl (p_recv q xs))); intros.
+    destruct H3. destruct H3. destruct H7. destruct H8. 
+  - specialize(_a23_bf p l e Q (p_send p l e Q) nil nil x0 H6 (eq_refl (p_send p l e Q))); intros.
+    destruct H10. destruct H10. destruct H10. destruct H11. 
+  - 
+  
+  admit.
+  
+  (* T-COND *)
+  inversion H. subst. 
+  inversion H1. subst. clear H1.
+  inversion H4. subst. clear H4. destruct H2. destruct H1. destruct H1. destruct H2.
+  inversion H2. subst. clear H2.
+  exists G. split.
+  apply t_sess; try easy. apply ForallT_par; try easy.
+  apply ForallT_mono; try easy. exists x. exists P.
+  split; try easy. split; try easy.
+  specialize(_a23_c (p_ite (e_val (vbool true)) P Q) (e_val (vbool true)) P Q x nil nil H3 (eq_refl (p_ite (e_val (vbool true)) P Q))); intros.
+  destruct H2. destruct H2. destruct H2. destruct H4. destruct H6.
+  apply tc_sub with (t := x0); try easy.
+  specialize(typable_implies_wfC H3); try easy.
+  apply multiC_refl.
+  
+  (* F-COND *)
+  inversion H. subst. 
+  inversion H1. subst. clear H1.
+  inversion H4. subst. clear H4. destruct H2. destruct H1. destruct H1. destruct H2.
+  inversion H2. subst. clear H2.
+  exists G. split.
+  apply t_sess; try easy. apply ForallT_par; try easy.
+  apply ForallT_mono; try easy. exists x. exists Q.
+  split; try easy. split; try easy.
+  specialize(_a23_c (p_ite (e_val (vbool false)) P Q) (e_val (vbool false)) P Q x nil nil H3 (eq_refl (p_ite (e_val (vbool false)) P Q))); intros.
+  destruct H2. destruct H2. destruct H2. destruct H4. destruct H6. destruct H7.
+  apply tc_sub with (t := x1); try easy.
+  specialize(typable_implies_wfC H3); try easy.
+  apply multiC_refl.
+  
+  (* R-STRUCT *)
+  specialize(_a22_2 M1 M1' G H2 H); intros.
+  specialize(IHbetaP G H3); intros. destruct IHbetaP. exists x. 
+  destruct H4. split; try easy.
+  specialize(_a22_2 M2' M2 x H4 H0); intros. easy.
+  
+Admitted.
