process/substitution_examples.v
@@ -9,7 +9,28 @@ Require Import Coq.Init.Datatypes.
 Require Import Coq.Arith.PeanoNat. 
 Require Import JMeq.
 
-Definition P := (p_rec (p_ite (e_var 0) (p_var 0) (p_var 1))).
+Definition E := e_var 0.
+Definition P := (p_ite E (p_var 0) (p_ite E (p_var 1) (p_rec (p_ite E (p_var 0) (p_ite E (p_var 1) (p_var 2)))))).
+
+Example subst2 : forall T, substitutionP 0 0 0 (p_rec P) P T -> False.
+Proof.
+  intros.
+  inversion H; subst. 
+  inversion H8; subst; try easy.
+  inversion H9; subst; try easy.
+  inversion H10; subst; try easy.
+  inversion H11; subst; try easy.
+  inversion H7; subst; try easy.
+  inversion H15; subst; try easy.
+  inversion H16; subst; try easy.
+  inversion H18; subst; try easy.
+  inversion H19; subst; try easy.
+  clear H9 H11 H15 H16 H7 H18 H19.
+  simpl in H.
+  
+  
+  
+  
 
 Example subst1 : substitutionP 0 0 0 P (p_ite (e_var 2) (p_rec (p_ite (e_var 1) (p_var 0) (p_var 1))) (p_var 0)) 
                                        (p_ite (e_var 2) (p_rec (p_ite (e_var 1) (p_var 0) (p_rec (p_ite (e_var 0) (p_var 0) (p_var 2))))) P).
