tree/inversion.v
@@ -1,0 +1,6 @@
+From SST Require Export tree.global tree.local.
+Require Import List String.
+Open Scope string_scope.
+
+
+
